% Equation 1
\begin{dmath}
{y}={k}^{{\alpha}}
\end{dmath}
% Equation 2
\begin{dmath}
{r}={\alpha}\, {k}^{{\alpha}-1}-{\delta}
\end{dmath}
% Equation 3
\begin{dmath}
{w}={k}^{{\alpha}}\, \left(1-{\alpha}\right)
\end{dmath}
% Equation 4
\begin{dmath}
{cy}={w}-{x}-{k}
\end{dmath}
% Equation 5
\begin{dmath}
{co}={x}\, \left(1+exp\left({z}\right)\, {g}\right)+{k}\, \left(1+{r}\right)
\end{dmath}
% Equation 6
\begin{dmath}
{cy}^{\left(-{\gamma}\right)}=\left(1+{r}\right)\, {\beta}\, {co}^{\left(-{\gamma}\right)}
\end{dmath}
% Equation 7
\begin{dmath}
{k}^{{\alpha}}={x}+{k}+{cy}+{co}
\end{dmath}
% Equation 8
\begin{dmath}
{z}={g}\, \left(1-{rho}\right)+{z}\, {rho}-{e}
\end{dmath}
