% Equation 1
\begin{dmath}
{y_{t}}={k_{t}}^{{\alpha}}
\end{dmath}
% Equation 2
\begin{dmath}
{r_{t}}={\alpha}\, {k_{t}}^{{\alpha}-1}-{\delta}
\end{dmath}
% Equation 3
\begin{dmath}
{w_{t}}={k_{t}}^{{\alpha}}\, \left(1-{\alpha}\right)
\end{dmath}
% Equation 4
\begin{dmath}
{cy_{t}}={w_{t}}-{x_{t}}-{k_{t}}
\end{dmath}
% Equation 5
\begin{dmath}
{co_{t}}={x_{t}}\, \left(1+exp\left({z_{t+1}}\right)\, {g}\right)+{k_{t}}\, \left(1+{r_{t}}\right)
\end{dmath}
% Equation 6
\begin{dmath}
{cy_{t}}^{\left(-{\gamma}\right)}={\beta}\, \left(1+{r_{t+1}}\right)\, {co_{t+1}}^{\left(-{\gamma}\right)}
\end{dmath}
% Equation 7
\begin{dmath}
{k_{t}}^{{\alpha}}={x_{t}}+{k_{t}}+{cy_{t}}+{co_{t}}
\end{dmath}
% Equation 8
\begin{dmath}
{z_{t}}={g}\, \left(1-{rho}\right)+{rho}\, {z_{t-1}}-{e_{t}}
\end{dmath}
